ToCoq.v
@@ -1,10 +1,9 @@
-Require Import Defs Mix.
+Require Import Defs Mix Proofs Meta Omega.
 Import ListNotations.
 Local Open Scope bool_scope.
 Local Open Scope lazy_bool_scope.
 Local Open Scope string_scope.
 Local Open Scope eqb_scope.
-
 
 Fixpoint arity_fun A n B :=
   match n with
@@ -12,8 +11,26 @@ Fixpoint arity_fun A n B :=
   | S n => A -> (arity_fun A n B)
   end.
 
-Definition model_funs A := string -> option { n:nat & arity_fun A n A }.
-Definition model_preds A := string -> option { n:nat & arity_fun A n Prop }.
+Definition get_arity {A B} (o : option { n:nat & arity_fun A n B}) :=
+  match o with
+  | None => None
+  | Some (existT _ n _) => Some n
+  end.
+
+Definition modfuns M := string -> option { n:nat & arity_fun M n M }.
+Definition modpreds M := string -> option { n:nat & arity_fun M n Prop }.
+
+Section SIGN.
+ Variable sign : gen_signature.
+ Variable M:Type.
+ Variable funs : modfuns M.
+ Variable preds : modpreds M.
+
+ Definition Adequate :=
+  (exists m:M, Logic.True) /\
+  (forall s, sign.(gen_fun_symbs) s = get_arity (funs s)) /\
+  (forall s, sign.(gen_pred_symbs) s = get_arity (preds s)).
+
 
 Definition optbind {A B} (o:option A)(f:A->option B) : option B :=
  match o with
@@ -31,10 +48,10 @@ Definition build_args {A B} :=
     | _, _ => fun _ => None
     end.
 
-Definition eval_term {A} (funs: model_funs A) genv lenv :=
+Definition eval_term genv lenv :=
   fix eval t :=
     match t with
-    | FVar x => list_assoc x genv
+    | FVar x => Some (genv x)
     | BVar n => nth_error lenv n
     | Fun f args => funs f >>= (fun '(existT _ n f) =>
                                   build_args n (List.map eval args) f)
@@ -47,7 +64,7 @@ Definition eval_op o :=
  | Imp => (fun p q : Prop => p -> q)
  end.
 
-Definition eval_form {A} (funs: model_funs A)(preds:model_preds A) genv :=
+Definition eval_form genv :=
   fix eval lenv f :=
     match f with
     | True => Logic.True
@@ -56,37 +73,313 @@ Definition eval_form {A} (funs: model_funs A)(preds:model_preds A) genv :=
     | Op o f1 f2 => eval_op o (eval lenv f1) (eval lenv f2)
     | Pred p args =>
       let optp := preds p >>= fun '(existT _ n f) =>
-                  build_args n (List.map (eval_term funs genv lenv) args) f
+                  build_args n (List.map (eval_term genv lenv) args) f
       in match optp with
          | Some p => p
          | None => Logic.False
          end
-    | Quant All f => forall (a:A), eval (a::lenv) f
-    | Quant Ex f => exists (a:A), eval (a::lenv) f
+    | Quant All f => forall (m:M), eval (m::lenv) f
+    | Quant Ex f => exists (m:M), eval (m::lenv) f
     end.
 
-Definition eval_ctx {A} (funs:model_funs A) preds genv lenv l :=
-  List.Forall (eval_form funs preds genv lenv) l.
+Definition eval_ctx genv lenv l :=
+  forall f, In f l -> eval_form genv lenv f.
 
-Definition eval_seq {A} (funs: model_funs A) preds genv lenv '(Γ⊢C) :=
-  eval_ctx funs preds genv lenv Γ /\
-  eval_form funs preds genv lenv C.
+Definition eval_seq genv lenv '(Γ⊢C) :=
+  eval_ctx genv lenv Γ ->
+  eval_form genv lenv C.
 
+Lemma max_0 n m : Nat.max n m = 0 <-> n=0 /\ m=0.
+Proof.
+ omega with *.
+Qed.
 
-Lemma correctness (sign:signature) {A} (funs:model_funs A) preds d :
- valid_deriv Intuiti d = true ->
-(* check_deriv d = true ->
- closed_deriv d = true ->
- adequate funs preds signature -> *)
- forall genv,
-   eval_seq funs preds genv [] (dseq d).
-Admitted.
+Lemma list_max_0 l : list_max l = 0 <-> forall n, In n l -> n = 0.
+Proof.
+ induction l; simpl; rewrite ?max_0 in *; intuition.
+Qed.
 
-Lemma correctness2 (sign:signature) {A} (funs:model_funs A) preds d :
- valid_deriv Classic d = true ->
-(* check_deriv d = true ->
- closed_deriv d = true ->
- adequate funs preds signature -> *)
- forall genv,
-   (forall P:Prop, P\/~P) -> eval_seq funs preds genv [] (dseq d).
-Admitted.
+Lemma build_args_uncheck {A B} n l (f:arity_fun A n B) :
+  List.length l <> n \/ In None l <-> build_args n l f = None.
+Proof.
+ revert n l f.
+ induction n; destruct l as [|o l]; cbn; intros f; auto.
+ - intuition easy.
+ - intuition easy.
+ - intuition easy.
+ - destruct o. rewrite <- IHn; intuition; easy. intuition.
+Qed.
+
+Lemma eval_term_notNone :
+ Adequate ->
+ forall genv (t:term),
+ check sign t = true /\ closed t = true <->
+  eval_term genv [] t <> None.
+Proof.
+ intros (_ & AD & _) genv.
+ fix IH 1. destruct t; cbn; auto; try easy.
+ - destruct n; cbn in *; intuition.
+ - rewrite AD. destruct (funs f) as [(n,fn)|]; cbn; [|intuition].
+   case eqbspec; intro LN.
+   + clear f.
+     assert (E : build_args n (map (eval_term genv []) l) fn <> None
+             <-> ~In None (map (eval_term genv []) l)).
+     { rewrite <- build_args_uncheck, map_length. intuition. }
+     rewrite E; clear E.
+     clear n fn LN. rewrite eqb_eq. revert l.
+     fix IH' 1. destruct l; cbn; auto.
+     intuition.
+     rewrite andb_true_iff, max_0.
+     specialize (IH' l). specialize (IH t).
+     unfold closed in IH. rewrite eqb_eq in IH.
+     intuition.
+   + rewrite <- build_args_uncheck, map_length. intuition.
+Qed.
+
+Lemma eval_term_ext genv genv' lenv t :
+ (forall v, Vars.In v (fvars t) -> genv v = genv' v) ->
+ eval_term genv lenv t = eval_term genv' lenv t.
+Proof.
+ revert t.
+ fix IH 1. destruct t; cbn; auto.
+ - intros. f_equal. apply H. varsdec.
+ - intros. case (funs f) as [(n,fn)|]; cbn; auto. clear f.
+   f_equal. clear n fn. revert l H.
+   fix IH' 1. destruct l; cbn; auto.
+   intros E. f_equal; auto with set.
+Qed.
+
+Lemma eval_form_ext genv genv' lenv f :
+ (forall v, Vars.In v (fvars f) -> genv v = genv' v) ->
+ eval_form genv lenv f <-> eval_form genv' lenv f.
+Proof.
+ revert lenv.
+ induction f; cbn; auto; intros; f_equal; auto with set.
+ - case (preds p) as [(n,fn)|]; cbn; [|reflexivity]; clear p.
+   assert (E : map (eval_term genv lenv) l =
+               map (eval_term genv' lenv) l).
+   { clear n fn.
+     revert l H.
+     induction l; cbn; auto.
+     intros E. f_equal; auto with set. apply eval_term_ext.
+     auto with set. }
+   now rewrite E.
+ - rewrite IHf; intuition.
+ - destruct o; cbn; rewrite IHf1, IHf2; intuition.
+ - destruct q.
+   + split; intros Hm m;
+     [rewrite <-IHf|rewrite IHf]; auto with set.
+   + split; intros (m,Hm); exists m;
+     [rewrite <-IHf|rewrite IHf]; auto with set.
+Qed.
+
+Lemma eval_ctx_ext genv genv' lenv c :
+ (forall v, Vars.In v (fvars c) -> genv v = genv' v) ->
+ eval_ctx genv lenv c <-> eval_ctx genv' lenv c.
+Proof.
+ intros E.
+ unfold eval_ctx.
+ split; intros H f Hf.
+ rewrite <- (eval_form_ext genv); auto with set.
+ intros v Hv. apply E. unfold fvars, fvars_list.
+ rewrite vars_unionmap_in. exists f. now split.
+ rewrite (eval_form_ext genv); auto with set.
+ intros v Hv. apply E. unfold fvars, fvars_list.
+ rewrite vars_unionmap_in. exists f. now split.
+Qed.
+
+Lemma eval_term_more_lenv genv lenv lenv' t :
+ eval_term genv lenv t <> None ->
+ eval_term genv (lenv++lenv') t = eval_term genv (lenv) t.
+Proof.
+ revert t.
+ fix IH 1. destruct t; cbn in *; intros H.
+ - reflexivity.
+ - rewrite nth_error_app1; trivial.
+   now apply nth_error_Some.
+ - case (funs f) as [(k,fk)|]; cbn in *; auto.
+   f_equal.
+   assert (H' : ~In None (map (eval_term genv lenv) l)).
+   { rewrite <- build_args_uncheck in H. intuition. }
+   clear H k fk f.
+   revert l H'.
+   fix IH' 1. destruct l; cbn; auto.
+   intros H. f_equal; auto.
+Qed.
+
+Lemma eval_term_bsubst genv lenv u m n t :
+ (level t <= S n)%nat ->
+ (List.length lenv = n) ->
+ eval_term genv [] u = Some m ->
+ eval_term genv (lenv++[m]) t = eval_term genv lenv (bsubst n u t).
+Proof.
+ revert t.
+ fix IH 1. destruct t; cbn; auto; intros LE Hn Hu.
+ - case eqbspec; intros.
+   + rewrite nth_error_app2; try omega.
+     replace (n0 - length lenv) with 0 by omega. simpl.
+     rewrite <- Hu. symmetry.
+     apply (eval_term_more_lenv genv [] lenv). now rewrite Hu.
+   + apply nth_error_app1. omega.
+ - case (funs f) as [(k,fk)|]; cbn; auto. f_equal. clear f k fk.
+   revert l LE Hn.
+   fix IH' 1. destruct l; cbn; auto.
+   intros LE Hn. f_equal.
+   apply IH; auto. omega with *.
+   apply IH'; auto. omega with *.
+Qed.
+
+Lemma eval_form_bsubst genv lenv u m n f :
+ (level f <= S n)%nat ->
+ (List.length lenv = n) ->
+ eval_term genv [] u = Some m ->
+ eval_form genv (lenv++[m]) f <-> eval_form genv lenv (bsubst n u f).
+Proof.
+ revert n lenv.
+ induction f; cbn; auto; intros; f_equal; auto with set.
+ - case (preds p) as [(k,fk)|]; cbn; [|reflexivity]; clear p.
+   assert (E : map (eval_term genv (lenv++[m])) l =
+               map (eval_term genv lenv) (map (bsubst n u) l)).
+   { clear k fk.
+     revert l H H0.
+     induction l; cbn; auto.
+     intros LE E. f_equal.
+     apply eval_term_bsubst; auto. omega with *.
+     apply IHl; auto. omega with *. }
+   now rewrite E.
+ - rewrite (IHf n); intuition.
+ - destruct o; cbn; rewrite (IHf1 n), (IHf2 n); intuition; omega with *.
+ - destruct q.
+   + split; intros Hm' m'.
+     * rewrite <-IHf; cbn; auto with set. omega with *.
+     * change (m'::(lenv++[m]))%list with ((m'::lenv)++[m])%list.
+       rewrite IHf; auto with set. omega with *. simpl; auto.
+   + split; intros (m',Hm'); exists m'.
+     * rewrite <-IHf; cbn; auto with set. omega with *.
+     * change (m'::(lenv++[m]))%list with ((m'::lenv)++[m])%list.
+       erewrite IHf; eauto with set. omega with *. simpl; auto.
+Qed.
+
+Lemma eval_form_bsubst0 genv u m f :
+ (level f <= 1)%nat ->
+ eval_term genv [] u = Some m ->
+ eval_form genv [m] f <-> eval_form genv [] (bsubst 0 u f).
+Proof.
+ intros LE.
+ now apply (eval_form_bsubst genv [] u m 0 f).
+Qed.
+
+Lemma eval_form_bsubst_adhoc genv m x f :
+ (level f <= 1)%nat ->
+ ~Vars.In x (fvars f) ->
+ eval_form genv [m] f <->
+ eval_form (fun v => if v =? x then m else genv v) []
+  (bsubst 0 (FVar x) f).
+Proof.
+ intros.
+ rewrite <- eval_form_bsubst0 with (m:=m); auto.
+ - apply eval_form_ext. intros v Hv.
+   case eqbspec; auto. intros ->. varsdec.
+ - cbn. now rewrite eqb_refl.
+Qed.
+
+Definition eval_logic lg :=
+ match lg with
+ | Classic => forall A:Prop, A\/~A
+ | Intuiti => Logic.True
+ end.
+
+Lemma correctness :
+ Adequate ->
+ forall (d:derivation) logic genv,
+ eval_logic logic ->
+ check sign d = true ->
+ closed d = true ->
+ valid_deriv logic d = true ->
+ eval_seq genv [] (dseq d).
+Proof.
+ intros AD.
+ induction d as [r s ds IH] using derivation_ind'.
+ cbn - [valid_deriv_step].
+ intros logic genv.
+ rewrite !lazy_andb_iff. rewrite eqb_eq, !max_0.
+ intros LG ((Cr,Cs),Cds) (Lr&Ls&Lds) (V,Vds).
+ assert (IH' : Forall (fun d => forall genv, eval_seq genv [] (dseq d)) ds).
+ { rewrite Forall_forall, forallb_forall in *.
+   rewrite list_max_0 in Lds.
+   intros d Hd genv'. eapply IH; eauto.
+   unfold closed. rewrite eqb_eq. apply Lds. now apply in_map. }
+ clear IH Cds Vds. mytac; cbn in *; intros Hc.
+ - now apply Hc, list_mem_in.
+ - destruct (H1 genv); auto.
+ - intro Hf. apply (H1 genv).
+   intros ? [<-|E]; auto.
+ - apply (H6 genv); auto.
+ - intuition.
+ - apply (H genv); auto.
+ - apply (H genv); auto.
+ - intuition.
+ - intuition.
+ - destruct (H4 genv); auto.
+   + apply (H6 genv). intros ? [<-|E]; auto.
+   + apply (H5 genv). intros ? [<-|E]; auto.
+ - intros Hf1. apply (H2 genv). intros ? [<-|E]; auto.
+ - apply (H1 genv); auto.
+ - intros m.
+   rewrite <- not_false_iff_true, negb_false_iff in H0.
+   rewrite Vars.mem_spec in H0.
+   rewrite eval_form_bsubst_adhoc with (x:=v).
+   apply H4.
+   rewrite <- (eval_ctx_ext genv); auto.
+   intros y Hy. case eqbspec; auto. intros <-. varsdec.
+   omega with *.
+   varsdec.
+ - assert (Hwit := eval_term_notNone AD genv wit).
+   destruct (eval_term genv [] wit) as [m|] eqn:E.
+   + rewrite <- eval_form_bsubst0 with (m:=m); auto.
+     rewrite !max_0 in Lds. intuition.
+   + unfold closed in Hwit. rewrite eqb_eq in Hwit. intuition.
+ - assert (Hwit := eval_term_notNone AD genv wit).
+   destruct (eval_term genv [] wit) as [m|] eqn:E.
+   + exists m.
+     rewrite eval_form_bsubst0 with (u:=wit); auto.
+     rewrite !max_0 in Ls. intuition.
+   + unfold closed in Hwit. rewrite eqb_eq in Hwit. intuition.
+ - destruct (H3 genv) as (m & Hm); auto.
+   rewrite <- not_false_iff_true, negb_false_iff in H0.
+   rewrite Vars.mem_spec in H0.
+   rewrite eval_form_bsubst_adhoc with (x:=v) in Hm.
+   erewrite eval_form_ext.
+   eapply H5.
+   intros A [<-|HA]. eapply Hm.
+   rewrite <- (eval_form_ext genv); auto.
+   intros y Hy. case eqbspec; auto. intros ->.
+   assert (Vars.In v (fvars c)).
+   { unfold fvars, fvars_list. rewrite vars_unionmap_in.
+     exists A; now split. }
+   varsdec.
+   intros y Hy. cbn. case eqbspec; auto. intros ->. varsdec.
+   rewrite !max_0 in Lds. intuition.
+   varsdec.
+ - destruct (LG (eval_form genv [] f0)); auto.
+   destruct (H genv). intros A [<-|HA]; auto.
+Qed.
+
+Lemma coherence :
+ Adequate ->
+ forall (d:derivation) logic,
+ eval_logic logic ->
+ check sign d = true ->
+ closed d = true ->
+ valid_deriv logic d = true ->
+ dseq d <> ([]⊢False)%form.
+Proof.
+ intros AD d logic LG CH CL VD E.
+ case AD. intros (m,_) _.
+ set (genv := fun (_:variable) => m).
+ assert (eval_seq genv [] (dseq d)).
+ { apply correctness with logic; auto. }
+ rewrite E in H. cbn in *. apply H. intros A. destruct 1.
+Qed.
+
+End SIGN.
